PropositionalDynamicLogic/ProofTheory/PropositionalDynamicLogic.v
@@ -21,20 +21,122 @@ Import PropositionalDynamicLanguageNotation.
 
 Check forall x y, |-- y --> x --> x.
 Check forall x y pi, |-- [pi] (x --> y) --> ( [pi]x --> [pi]y ).
-Check forall x p q, |-- [p-q] x <--> [p][q]x.
+Check forall x p q, |-- [p -;- q] x <--> [p][q]x.
 Check forall x p q, |-- [p\\//q] x <--> [p]x || [q]x.
 Check forall x pi, |-- [pi*]x <--> (x || [pi][pi*]x ).
 Check forall x pi, |-- [pi*](x --> [pi]x) --> (x --> [pi*]x).
 
 Class PropositionalDynamicLogicK 
 (L: Language){minL: MinimunLanguage L}{pL: PropositionalLanguage L}
-(Gamma: ProofTheory L){minAX: MinimunAxiomatization L Gamma}{ipGamma: IntuitionisticPropositionalLogic L Gamma} 
-(Pro: Program){ProOp: ProgramOperation Pro}{pdL: PropositionalDynamicLanguage L Pro} := {
+(Pro: Program){ProOp: ProgramOperation Pro}{pdL: PropositionalDynamicLanguage L Pro}
+(Gamma: ProofTheory L)
+{minAX: MinimunAxiomatization L Gamma}
+{ipGamma: IntuitionisticPropositionalLogic L Gamma}
+{cpGamma: ClassicalPropositionalLogic L Gamma} 
+ := {
   axiom_K: forall x y pi, |-- [pi] (x --> y) --> ( [pi]x --> [pi]y );
   axiom_choice: forall x p q, |-- [p\\//q] x <--> [p]x || [q]x;
-  axiom_composition: forall x p q, |-- [p-q]x <--> [p][q]x;
+  axiom_composition: forall x p q, |-- [p-;-q]x <--> [p][q]x;
   axiom_iteration: forall x pi, |-- [pi*]x <--> (x || [pi][pi*]x );
   axiom_induction: forall x pi, |-- [pi*](x --> [pi]x) --> (x --> [pi*]x)
 }.
 
+
+
+Class PropositionalDynamicSequentCalculusK 
+(L: Language) {minL: MinimunLanguage L} {pL: PropositionalLanguage L}
+(Pro: Program){ProOp: ProgramOperation Pro}{pdL: PropositionalDynamicLanguage L Pro}
+(Gamma: ProofTheory L) 
+{bSC: BasicSequentCalculus L Gamma} 
+{minSC: MinimunSequentCalculus L Gamma} 
+{ipSC: IntuitionisticPropositionalSequentCalculus L Gamma}
+{cpGamma: ClassicalPropositionalSequentCalculus L Gamma} := {
+  deduction_axiom_K: forall Phi x y pi, Phi |-- [pi](x --> y) -> Phi |-- [pi]x --> [pi]y
+}.
+
+
+Goal  forall (L: Language){minL: MinimunLanguage L}{pL: PropositionalLanguage L}
+(Gamma: ProofTheory L){minAX: MinimunAxiomatization L Gamma}{ipGamma: IntuitionisticPropositionalLogic L Gamma} 
+(Pro: Program){ProOp: ProgramOperation Pro}{pdL: PropositionalDynamicLanguage L Pro}  
+x y pi, |-- [pi](x --> y --> x).
+
+intros.
+pose proof axiom1 x y. Abort.
+
 Check axiom_K.
+
+Section DerivableRulesFromSequentCalculus1.
+Context {L: Language}
+        {Pro: Program}
+        {ProOp: ProgramOperation Pro}
+        {minL: MinimunLanguage L}
+        {pL: PropositionalLanguage L}
+        {pdL: PropositionalDynamicLanguage L Pro}
+        {Gamma: ProofTheory L}
+        {SC: NormalSequentCalculus L Gamma}
+        {bSC: BasicSequentCalculus L Gamma}
+        {minSC: MinimunSequentCalculus L Gamma}
+        {ipSC: IntuitionisticPropositionalSequentCalculus L Gamma}
+        {cpSC: ClassicalPropositionalSequentCalculus L Gamma}
+        {pdSC: PropositionalDynamicSequentCalculusK L Pro Gamma}
+        .
+
+
+Lemma derivable_axiom_K: forall Phi x y pi, Phi |-- [pi] (x --> y) --> ( [pi]x --> [pi]y ).
+Proof.
+  intros.
+  rewrite <- deduction_theorem.
+  apply deduction_axiom_K.
+  
+  pose proof (deduction_axiom_K (Empty_set _) x y pi).
+  
+  
+
+Lemma derivable_axiom_choice: forall x p q, |-- [p\\//q] x <--> [p]x || [q]x.
+Proof. Admitted.
+
+Lemma derivable_axiom_composition: forall x p q, |-- [p-;-q]x <--> [p][q]x.
+Proof. Admitted.
+
+Lemma derivable_axiom_iteration: forall x pi, |-- [pi*]x <--> (x || [pi][pi*]x ).
+Proof. Admitted.
+
+Lemma derivable_axiom_induction: forall x pi, |-- [pi*](x --> [pi]x) --> (x --> [pi*]x).
+Proof. Admitted.
+
+
+End DerivableRulesFromSequentCalculus1.
+
+Section SequentCalculus2Axiomatization.
+
+Context {L: Language}
+        {Pro: Program}
+        {ProOp: ProgramOperation Pro}
+        {minL: MinimunLanguage L}
+        {pL: PropositionalLanguage L}
+        {pdL: PropositionalDynamicLanguage L Pro}
+        {Gamma: ProofTheory L}
+        {SC: NormalSequentCalculus L Gamma}
+        {bSC: BasicSequentCalculus L Gamma}
+        {minSC: MinimunSequentCalculus L Gamma}
+        {ipSC: IntuitionisticPropositionalSequentCalculus L Gamma}
+        {cpSC: ClassicalPropositionalSequentCalculus L Gamma}
+        {pdSC: PropositionalDynamicSequentCalculusK L Pro Gamma}
+        {minAX: MinimunAxiomatization L Gamma}
+        {ipAX: IntuitionisticPropositionalLogic L Gamma}
+        {cpAX: ClassicalPropositionalLogic L Gamma}
+        .
+
+Lemma SequentCalculus2Axiomatization_pdSC: PropositionalDynamicLogicK L Pro Gamma.
+Proof.
+  intros.
+  constructor.
+  - apply derivable_axiom_K.
+  - apply derivable_axiom_choice.
+  - apply derivable_axiom_composition.
+  - apply derivable_axiom_iteration.
+  - apply derivable_axiom_induction.
+Qed.
+
+End SequentCalculus2Axiomatization.
+
