PropositionalDynamicLogic/Semantics/Kripke.v
@@ -11,22 +11,66 @@ Local Open Scope kripke_model.
 Import PropositionalDynamicLanguageNotation.
 Import KripkeModelFamilyNotation.
 
+
+Module PDL_KM.
+
+Class Relation (prog: Type)(worlds: Type): Type :=
+  Krelation: prog -> worlds -> worlds -> Prop.
+
+End PDL_KM.
+
+
 Module Semantics.
 
-Class Relation (worlds: Type)(Pro: Program): Type :=
-  Krelation: program -> worlds -> worlds -> Prop.
-
-Definition boxp {worlds: Type}{Pro: Program}{R: Relation worlds Pro}
-(pi: program)(X: Ensemble worlds): Ensemble worlds :=
-fun m => forall n, Krelation pi m n -> X n.
+Definition boxp {prog: Type}{worlds: Type}{R: PDL_KM.Relation prog worlds}
+(pi: prog)(X: Ensemble worlds): Ensemble worlds :=
+fun m => forall n, PDL_KM.Krelation pi m n -> X n.
 
 End Semantics.
+Locate Kdenotation. Print Kdenotation.
 
-Class KripkeModalSemantics 
+Class KripkePropositionalDynamicSemantics 
 (L: Language) {minL: MinimunLanguage L} {pL: PropositionalLanguage L}
 (Pro: Program) {pdL: PropositionalDynamicLanguage L Pro} 
 (MD: Model) {kMD: KripkeModel MD} 
-(M: Kmodel) {R: Relation (Kworlds M)} 
+(M: Kmodel) 
+{R: PDL_KM.Relation (program) (Kworlds M)} 
 (SM: Semantics L MD): Type := {
+
+  denote_boxp: forall (pi:program) (x: expr), Same_set _ (Kdenotation M ([pi] x) ) (Semantics.boxp pi (Kdenotation M x) )
   
 }.
+Print KripkeModel.
+Lemma sat_boxp 
+{L:Language}{minL: MinimunLanguage L}{pL: PropositionalLanguage L}
+{Pro: Program}{pdL: PropositionalDynamicLanguage L Pro}
+{MD: Model}{kMD: KripkeModel MD}{M:Kmodel}
+{R: PDL_KM.Relation program (Kworlds M)}
+{SM: Semantics L MD}{kpdSM: KripkePropositionalDynamicSemantics L Pro MD M SM}:
+forall m x pi, KRIPKE: M, m |= [pi] x <-> (forall n, PDL_KM.Krelation pi m n -> KRIPKE: M, n |= x).
+Proof.
+  intros.
+  unfold satisfies.
+  pose proof denote_boxp pi x as H.
+  destruct H as [H1 H2].
+  split. unfold Semantics.boxp in H1. unfold Included in H1. unfold Ensembles.In in H1.
+  - apply (H1 m).
+  - apply (H2 m).
+Qed.
+
+
+
+
+
+
+
+
+
+
+
+
+
+
+
+
+
