PropositionalDynamicLogic/Complete/Fischer_Ladner_Closure.v
@@ -1,0 +1,247 @@
+
+Require Import Logic.GeneralLogic.Base.
+Require Import Logic.GeneralLogic.ProofTheory.BasicSequentCalculus.
+Require Import Logic.MinimunLogic.Syntax.
+Require Import Logic.MinimunLogic.ProofTheory.Minimun.
+Require Import Logic.MinimunLogic.ProofTheory.RewriteClass.
+Require Import Logic.MinimunLogic.ProofTheory.ProofTheoryPatterns.
+Require Import Logic.PropositionalLogic.Syntax.
+Require Import Logic.PropositionalLogic.ProofTheory.Intuitionistic.
+Require Import Logic.PropositionalLogic.ProofTheory.GodelDummett.
+Require Import Logic.PropositionalLogic.ProofTheory.DeMorgan.
+Require Import Logic.PropositionalLogic.ProofTheory.Classical.
+Require Import Logic.PropositionalLogic.ProofTheory.RewriteClass.
+Require Import Logic.PropositionalLogic.ProofTheory.ProofTheoryPatterns.
+Require Import Logic.PropositionalDynamicLogic.Syntax.
+
+
+Import PropositionalDynamicLanguageNotation.
+
+Require Import Coq.Sets.Ensembles.
+
+Section Fischer_Ladner_Closed.
+
+
+Context {L: Language}
+        {Pro: Program}
+        {ProOp: ProgramOperation L Pro}
+        {minL: MinimunLanguage L}
+        {pL: PropositionalLanguage L}
+        {pdL: PropositionalDynamicLanguage L Pro}
+
+        .
+
+Record FL_closed (X: Ensemble expr):Prop :={
+  FL_closed_impp: forall x y, In expr X (impp x y) -> In _ X x /\ In _ X y;
+  FL_closed_orp: forall x y, In _ X (orp x y) -> In _ X x /\ In _ X y;
+  FL_closed_andp: forall x y, In _ X (andp x y) -> In _ X x /\ In _ X y;
+  FL_closed_falsep: In _ X (falsep);
+  FL_closed_boxp: forall x pi, In _ X (boxp pi x) -> In _ X x;
+  FL_closed_boxp_choice: forall x p q, In _ X (boxp (choice p q) x) -> In _ X (orp (boxp p x) (boxp q x));
+  FL_closed_boxp_composition: forall x p q, In _ X (boxp (composition p q) x) -> In _ X (boxp p (boxp q x));
+  FL_closed_boxp_iteration: forall x pi, In _ X (boxp (iteration pi) x) -> In _ X (boxp pi (boxp (iteration pi) x));
+  FL_closed_boxp_test: forall x y, In _ X (boxp (test y) x) -> In _ X x /\  In _ X y;
+}.
+
+Class FL_closed_set: Type :={
+  FL_closure_construction (psi: expr): Ensemble expr
+}.
+
+Definition FL_closure_construction_is_FL_closed (flc: FL_closed_set): Prop := 
+forall psi, FL_closed (FL_closure_construction psi).
+
+Record FL_axiom {flc: FL_closed_set} (psi:expr) (A: Ensemble expr): Prop :={
+  FL_axiom_included: Included _ A (FL_closure_construction psi);
+  (* FL_axiom_consist: consistent A; *)
+  (* FL_axiom_MCS: forall B, Included _ B FL_closure_construction /\ Included _ A B -> ~ (consistent B);*)
+}.
+
+Definition FL_axiom_existence {flc: FL_closed_set}:Prop :=
+forall psi, exists A, FL_axiom psi A.
+
+End Fischer_Ladner_Closed.
+
+
+
+
+Require Import Logic.PropositionalDynamicLogic.DeepEmbedded.PropositionalDynamicLanguage.
+
+Section FL_closure.
+
+Context {Sigma: PropositionalVariables}
+        {ProV: ProgramVariables}.
+
+Fixpoint FL_closure (x: expr Sigma ProV): Ensemble (expr Sigma ProV):=
+  Union _ (Singleton _ x)
+  match x with
+  | impp y z => Union _ (FL_closure y) (FL_closure z)
+  | orp y z => Union _ (FL_closure y) (FL_closure z)
+  | andp y z => Union _ (FL_closure y) (FL_closure z)
+  | falsep => Singleton _ (falsep)
+  | boxp pi x => 
+      Union _ (Singleton _ x)
+      match pi with
+      | choice p q => Singleton _ (orp (boxp p x)(boxp q x))
+      | composition p q => Singleton _ (boxp p (boxp q x))
+      | iteration p => Singleton _ (boxp p (boxp pi x))
+      | test y => Singleton _ y
+      | basep p => Empty_set _
+      end
+  | varp v => Singleton _ (varp v)
+  end.
+
+
+
+Lemma FL_closure_include_self: forall x, In _ (FL_closure x) x.
+Proof.
+  intros x. 
+  destruct x; apply Union_introl; apply In_singleton.
+Qed.
+
+Lemma FL_closure_ensure_impp: 
+forall x y psi, In _ (FL_closure psi) (impp x y) ->
+In _ (FL_closure psi) x /\ In _ (FL_closure psi) y.
+Proof. 
+  induction psi.
+  - intros H. simpl in H.
+    remember (impp x y) as e. destruct H. 
+    + rewrite Heqe in H.
+      remember (impp x y) as f. destruct H. 
+      rewrite Heqf. split.
+      * simpl. apply Union_intror. apply Union_introl. apply FL_closure_include_self.
+      * simpl. apply Union_intror. apply Union_intror. apply FL_closure_include_self.
+    + rewrite Heqe in H.
+      remember (impp x y) as f. destruct H. 
+      * rewrite <- Heqe in H. split.
+        ** simpl. apply Union_intror. apply Union_introl. apply (IHpsi1 H).
+        ** simpl. apply Union_intror. apply Union_introl. apply (IHpsi1 H).
+      * rewrite <- Heqe in H. split.
+        ** simpl. apply Union_intror. apply Union_intror. apply (IHpsi2 H).
+        ** simpl. apply Union_intror. apply Union_intror. apply (IHpsi2 H).
+  (* almost the same *)
+  - admit.
+  - admit.
+  - admit.
+  - induction p.
+    + admit.
+    + admit.
+    + admit.
+    + admit.
+    + admit.
+  - intros H. simpl in H.
+    remember (impp x y) as e. destruct H.
+    + rewrite Heqe in H. remember (impp x y) as f. destruct H. inversion Heqf.
+    + rewrite Heqe in H. remember (impp x y) as f. destruct H. inversion Heqf.
+    
+Admitted.
+
+Lemma FL_closure_ensure_orp: 
+forall psi x y, In _ (FL_closure psi) (orp x y) ->
+In _ (FL_closure psi) x /\ In _ (FL_closure psi) y.
+Proof. Admitted.
+
+
+Lemma FL_closure_ensure_andp: 
+forall psi x y, In _ (FL_closure psi) (andp x y) ->
+In _ (FL_closure psi) x /\ In _ (FL_closure psi) y.
+Proof. Admitted.
+
+Lemma FL_closure_ensure_falsep: 
+forall psi, In _ (FL_closure psi) falsep.
+Proof. Admitted.
+
+Lemma FL_closure_ensure_boxp: 
+forall psi x pi , In _ (FL_closure psi) (boxp pi x) ->
+In _ (FL_closure psi) x.
+Proof. Admitted.
+
+Lemma FL_closure_ensure_boxp_choice: 
+forall psi x p q ,
+In (expr Sigma ProV) (FL_closure psi) (boxp (choice p q) x) ->
+In (expr Sigma ProV) (FL_closure psi) (orp (boxp p x) (boxp q x)).
+Proof. Admitted.
+
+Lemma FL_closure_ensure_boxp_composition: 
+forall psi x p q,
+In (expr Sigma ProV) (FL_closure psi) (boxp (composition p q) x) ->
+In (expr Sigma ProV) (FL_closure psi) (boxp p (boxp q x)).
+Proof. Admitted.
+
+Lemma FL_closure_ensure_boxp_iteration:
+forall psi x pi,
+In (expr Sigma ProV) (FL_closure psi) (boxp (iteration pi) x) ->
+In (expr Sigma ProV) (FL_closure psi) (boxp pi (boxp (iteration pi) x)).
+Proof. Admitted.
+
+Lemma FL_closure_ensure_boxp_test:
+forall psi x y,
+In (expr Sigma ProV) (FL_closure psi) (boxp (test y) x) ->
+In (expr Sigma ProV) (FL_closure psi) x /\
+In (expr Sigma ProV) (FL_closure psi) y.
+Proof. Admitted.
+
+End FL_closure.
+
+
+
+
+Section FL_closure_is_FL_closed.
+Context {Sigma: PropositionalVariables}
+        {ProV: ProgramVariables}
+        
+        .
+
+Instance L {Sigma: PropositionalVariables} {ProV: ProgramVariables}: Language 
+:= Build_Language (expr Sigma ProV).
+
+Instance Pro {Sigma: PropositionalVariables} {ProV: ProgramVariables}: Program
+:= Build_Program (program Sigma ProV).
+
+
+Instance ProOp {Sigma: PropositionalVariables} {ProV: ProgramVariables}: ProgramOperation L Pro
+:= Build_ProgramOperation L Pro choice composition iteration test.
+
+Instance minL {Sigma: PropositionalVariables} {ProV: ProgramVariables}: MinimunLanguage L
+:= Build_MinimunLanguage L impp.
+
+Instance pL {Sigma: PropositionalVariables} {Pro: ProgramVariables}: PropositionalLanguage L
+:= Build_PropositionalLanguage L andp orp falsep.
+
+Instance pdL {Sigma: PropositionalVariables} {ProV: ProgramVariables}: PropositionalDynamicLanguage L Pro
+:= Build_PropositionalDynamicLanguage L Pro boxp.
+
+Instance flc: FL_closed_set:= Build_FL_closed_set FL_closure.
+
+Lemma FL_closure_is_FL_closed: FL_closure_construction_is_FL_closed flc.
+Proof.
+  intros psi. constructor.
+  - intros x y. apply (FL_closure_ensure_impp x y psi).
+  - apply FL_closure_ensure_orp.
+  - apply FL_closure_ensure_andp.
+  - apply FL_closure_ensure_falsep.
+  - apply FL_closure_ensure_boxp.
+  - apply FL_closure_ensure_boxp_choice.
+  - apply FL_closure_ensure_boxp_composition.
+  - apply FL_closure_ensure_boxp_iteration.
+  - apply FL_closure_ensure_boxp_test.
+Qed.
+
+Lemma Lindenbaum_lemma: FL_axiom_existence.
+Proof.
+  hnf. intros.
+Admitted.
+
+
+End FL_closure_is_FL_closed.
+
+
+
+
+
+
+
+
+
+
+
+
