PropositionalDynamicLogic/Complete/Truth_Kripke.v
@@ -1,0 +1,48 @@
+Require Import Coq.Logic.FunctionalExtensionality.
+Require Import Coq.Logic.Classical_Prop.
+Require Import Coq.Logic.Classical_Pred_Type.
+Require Import Logic.lib.Bijection.
+Require Import Logic.lib.Countable.
+Require Import Logic.GeneralLogic.Base.
+Require Import Logic.GeneralLogic.KripkeModel.
+Require Import Logic.GeneralLogic.ProofTheory.BasicSequentCalculus.
+Require Import Logic.GeneralLogic.Semantics.Kripke.
+Require Import Logic.GeneralLogic.Complete.ContextProperty.
+Require Import Logic.GeneralLogic.Complete.ContextProperty_Kripke.
+Require Import Logic.MinimunLogic.Syntax.
+Require Import Logic.MinimunLogic.ProofTheory.Minimun.
+Require Import Logic.MinimunLogic.Semantics.Kripke.
+Require Import Logic.MinimunLogic.Complete.ContextProperty_Kripke.
+Require Import Logic.PropositionalLogic.Syntax.
+Require Import Logic.PropositionalLogic.ProofTheory.Intuitionistic.
+Require Import Logic.PropositionalLogic.ProofTheory.Classical.
+Require Import Logic.PropositionalLogic.Semantics.Kripke.
+Require Import Logic.PropositionalLogic.Complete.ContextProperty_Kripke.
+
+Require Import Logic.PropositionalDynamicLogic.Syntax.
+
+Local Open Scope logic_base.
+Local Open Scope syntax.
+Local Open Scope kripke_model.
+Import PropositionalLanguageNotation.
+Import KripkeModelFamilyNotation.
+
+Section TruthLemma.
+Locate ClassicalPropositionalSequentCalculus.
+
+Context {L: Language}
+        {minL: MinimunLanguage L}
+        {pL: PropositionalLanguage L}
+        {Gamma: ProofTheory L}
+        {bSC: BasicSequentCalculus L Gamma}
+        {minSC: MinimunSequentCalculus L Gamma}
+        {ipSC: IntuitionisticPropositionalSequentCalculus L Gamma}
+        {cpSC: ClassicalPropositionalSequentCalculus L Gamma}
+        {MD: Model}
+        {kMD: KripkeModel MD}
+        {M: Kmodel}
+        {R: Relation (Kworlds M)}
+        {SM: Semantics L MD}
+        {kminSM: KripkeMinimunSemantics L MD M SM}
+        {kpSM: KripkePropositionalSemantics L MD M SM}.
+
