PropositionalDynamicLogic/DeepEmbedded/KripkeSemantics.v
@@ -1,0 +1,46 @@
+Require Import Coq.Logic.Classical_Prop.
+Require Import Coq.Classes.RelationClasses.
+Require Import Coq.Relations.Relation_Definitions.
+Require Import Logic.lib.Ensembles_ext.
+Require Import Logic.GeneralLogic.Base.
+Require Import Logic.GeneralLogic.KripkeModel.
+Require Import Logic.GeneralLogic.Semantics.Kripke.
+Require Import Logic.MinimunLogic.Syntax.
+Require Import Logic.MinimunLogic.Semantics.Kripke.
+Require Import Logic.PropositionalLogic.Syntax.
+Require Import Logic.PropositionalLogic.Semantics.Kripke.
+Require Import Logic.PropositionalDynamicLogic.Syntax.
+Require Import Logic.PropositionalDynamicLogic.Semantics.Kripke.
+
+Require Import Logic.PropositionalDynamicLogic.DeepEmbedded.PropositionalDynamicLanguage.
+
+Locate PropositionalDynamicLanguage.
+Import PropositionalDynamicLanguage.
+
+Record frame: Type :={
+  underlying_set:> Type;
+  underlying_relation:> relation underlying_set;
+  
+  underlying_modal_relation: relation underlying_set
+}.
+
+Infix "<=" := (underlying_relation _): TheKripkeSemantics.
+Local Open Scope TheKripkeSemantics.
+
+Definition sem (f:frame) := @Ensemble (underlying_set f).
+
+Section KripkeSemantics.
+Context {Sigma: PropositionalVariables}
+        {ProV: ProgramVariables}.
+
+Definition denotation (F: frame) (eval: Var -> sem F): expr Sigma ProV -> sem F :=
+  fix denotation (x: expr Sigma ProV): sem F:=
+  match x with
+  | andp y z => @Semantics.andp F (denotation y) (denotation z)
+  | orp y z => @Semantics.orp F (denotation y) (denotation z)
+  | impp y z => @Semantics.impp F (underlying_relation F) (denotation y) (denotation z)
+  | falsep => @Semantics.falsep F
+  | boxp pi x=> @Semantics.boxp
+  | varp p => eval p
+  end.
+
